<?xml version="1.0"?>
<rdf:RDF xmlns="http://lari-datasets.ilc.cnr.it/lemonEty#"
     xml:base="http://lari-datasets.ilc.cnr.it/lemonEty"
     xmlns:dc="http://purl.org/dc/elements/1.1/"
     xmlns:ns="http://creativecommons.org/ns#"
     xmlns:dct="http://purl.org/dc/terms/"
     xmlns:ns1="http://www.w3.org/2003/06/sw-vocab-status/ns#"
     xmlns:owl="http://www.w3.org/2002/07/owl#"
     xmlns:rdf="http://www.w3.org/1999/02/22-rdf-syntax-ns#"
     xmlns:xml="http://www.w3.org/XML/1998/namespace"
     xmlns:xsd="http://www.w3.org/2001/XMLSchema#"
     xmlns:rdfs="http://www.w3.org/2000/01/rdf-schema#"
     xmlns:vann="http://purl.org/vocab/vann/">
    <owl:Ontology rdf:about="http://lari-datasets.ilc.cnr.it/lemonEty#">
        <owl:imports rdf:resource="http://www.w3.org/ns/lemon/all"/>
        <owl:imports rdf:resource="http://www.w3.org/ns/lemon/ontolex"/>
        <dct:contributor rdf:resource="http://www.ilc.cnr.it/en/content/anas_fahad_khan"/>
        <dct:description xml:lang="en">lemonEty is an extension of the ontolex-lemon model that provides concepts and properties that are useful in representing etymological information.</dct:description>
        <dct:issued>2018-05-04</dct:issued>
        <dct:rights>CC-BY</dct:rights>
        <dct:title xml:lang="en">lemonEty</dct:title>
        <owl:versionInfo>Version 0.1.0</owl:versionInfo>
    </owl:Ontology>
    


    <!-- 
    ///////////////////////////////////////////////////////////////////////////////////////
    //
    // Annotation properties
    //
    ///////////////////////////////////////////////////////////////////////////////////////
     -->

    


    <!-- http://purl.org/dc/terms/contributor -->

    <owl:AnnotationProperty rdf:about="http://purl.org/dc/terms/contributor"/>
    


    <!-- http://purl.org/dc/terms/description -->

    <owl:AnnotationProperty rdf:about="http://purl.org/dc/terms/description"/>
    


    <!-- http://purl.org/dc/terms/issued -->

    <owl:AnnotationProperty rdf:about="http://purl.org/dc/terms/issued"/>
    


    <!-- http://purl.org/dc/terms/rights -->

    <owl:AnnotationProperty rdf:about="http://purl.org/dc/terms/rights"/>
    


    <!-- http://purl.org/dc/terms/title -->

    <owl:AnnotationProperty rdf:about="http://purl.org/dc/terms/title"/>
    


    <!-- 
    ///////////////////////////////////////////////////////////////////////////////////////
    //
    // Object Properties
    //
    ///////////////////////////////////////////////////////////////////////////////////////
     -->

    


    <!-- http://lari-datasets.ilc.cnr.it/lemonEty#cognate -->

    <owl:ObjectProperty rdf:about="http://lari-datasets.ilc.cnr.it/lemonEty#cognate">
        <rdfs:range rdf:resource="http://lari-datasets.ilc.cnr.it/lemonEty#Cognate"/>
        <rdfs:comment xml:lang="en">&apos;cognate&apos; is an object property linking a linguistic entity with a Cognate.</rdfs:comment>
        <rdfs:label xml:lang="en">cognate</rdfs:label>
    </owl:ObjectProperty>
    


    <!-- http://lari-datasets.ilc.cnr.it/lemonEty#etyLinkType -->

    <owl:ObjectProperty rdf:about="http://lari-datasets.ilc.cnr.it/lemonEty#etyLinkType">
        <rdfs:range rdf:resource="http://lari-datasets.ilc.cnr.it/lemonEty#EtyLink"/>
    </owl:ObjectProperty>
    


    <!-- http://lari-datasets.ilc.cnr.it/lemonEty#etySource -->

    <owl:ObjectProperty rdf:about="http://lari-datasets.ilc.cnr.it/lemonEty#etySource">
        <rdfs:domain rdf:resource="http://lari-datasets.ilc.cnr.it/lemonEty#EtyLink"/>
        <rdfs:comment xml:lang="en">&apos;etymological source&apos; is an object property that links an EtyLink with a linguistic entity which is the source of the relationship which the former represents.</rdfs:comment>
        <rdfs:label xml:lang="en">etymological source</rdfs:label>
    </owl:ObjectProperty>
    


    <!-- http://lari-datasets.ilc.cnr.it/lemonEty#etySubSource -->

    <owl:ObjectProperty rdf:about="http://lari-datasets.ilc.cnr.it/lemonEty#etySubSource">
        <rdfs:domain rdf:resource="http://lari-datasets.ilc.cnr.it/lemonEty#EtyLink"/>
        <rdfs:comment xml:lang="en">&apos;etymological sub-source&apos; is an object property that further specifies the etymological source of an EtyLink (assuming a prior use of etySource).</rdfs:comment>
        <rdfs:label xml:lang="en">etymological sub-source</rdfs:label>
    </owl:ObjectProperty>
    


    <!-- http://lari-datasets.ilc.cnr.it/lemonEty#etySubTarget -->

    <owl:ObjectProperty rdf:about="http://lari-datasets.ilc.cnr.it/lemonEty#etySubTarget">
        <rdfs:domain rdf:resource="http://lari-datasets.ilc.cnr.it/lemonEty#EtyLink"/>
        <rdfs:comment xml:lang="en">&apos;etymological sub-target&apos; is an object property that further specifies the etymological target of an EtyLink (assuming a prior use of etyTarget).</rdfs:comment>
        <rdfs:label xml:lang="en">etymological sub-target</rdfs:label>
    </owl:ObjectProperty>
    


    <!-- http://lari-datasets.ilc.cnr.it/lemonEty#etyTarget -->

    <owl:ObjectProperty rdf:about="http://lari-datasets.ilc.cnr.it/lemonEty#etyTarget">
        <rdfs:domain rdf:resource="http://lari-datasets.ilc.cnr.it/lemonEty#EtyLink"/>
        <rdfs:comment xml:lang="en">&apos;etymological target&apos; is an object property that links an EtyLink with a linguistic entity which is the target of the relationship which the former represents.</rdfs:comment>
        <rdfs:label xml:lang="en">etymological target</rdfs:label>
    </owl:ObjectProperty>
    


    <!-- http://lari-datasets.ilc.cnr.it/lemonEty#etymology -->

    <owl:ObjectProperty rdf:about="http://lari-datasets.ilc.cnr.it/lemonEty#etymology">
        <rdfs:range rdf:resource="http://lari-datasets.ilc.cnr.it/lemonEty#Etymology"/>
        <rdfs:comment xml:lang="en">&apos;etymology&apos; is  an object property linking a linguistic entity with an Etymology.</rdfs:comment>
        <rdfs:label xml:lang="en">etymology</rdfs:label>
    </owl:ObjectProperty>
    


    <!-- http://lari-datasets.ilc.cnr.it/lemonEty#etymon -->

    <owl:ObjectProperty rdf:about="http://lari-datasets.ilc.cnr.it/lemonEty#etymon">
        <rdfs:domain rdf:resource="http://lari-datasets.ilc.cnr.it/lemonEty#Etymology"/>
        <rdfs:range rdf:resource="http://lari-datasets.ilc.cnr.it/lemonEty#Etymon"/>
        <rdfs:comment xml:lang="en">&apos;etymon&apos; is  an object property that relates an Etymology with its related etymons.</rdfs:comment>
        <rdfs:label xml:lang="en">etymon</rdfs:label>
    </owl:ObjectProperty>
    


    <!-- http://lari-datasets.ilc.cnr.it/lemonEty#hasEtyLink -->

    <owl:ObjectProperty rdf:about="http://lari-datasets.ilc.cnr.it/lemonEty#hasEtyLink">
        <rdfs:domain rdf:resource="http://lari-datasets.ilc.cnr.it/lemonEty#Etymology"/>
        <rdfs:range rdf:resource="http://lari-datasets.ilc.cnr.it/lemonEty#EtyLink"/>
        <rdfs:comment xml:lang="en">&apos;has etymological link&apos; is an object property that relates an Etymology with one of its constituent Etymological Link objects.</rdfs:comment>
        <rdfs:label xml:lang="en">has etymological link</rdfs:label>
    </owl:ObjectProperty>
    


    <!-- http://lari-datasets.ilc.cnr.it/lemonEty#isCognateOf -->

    <owl:ObjectProperty rdf:about="http://lari-datasets.ilc.cnr.it/lemonEty#isCognateOf">
        <rdfs:domain rdf:resource="http://lari-datasets.ilc.cnr.it/lemonEty#Cognate"/>
        <rdfs:comment xml:lang="en">&apos;is cognate of&apos; is an object property linking a Cognate with some linguistic entity.</rdfs:comment>
        <rdfs:label xml:lang="en">isCognateOf</rdfs:label>
    </owl:ObjectProperty>
    


    <!-- http://lari-datasets.ilc.cnr.it/lemonEty#isEtyLinkOf -->

    <owl:ObjectProperty rdf:about="http://lari-datasets.ilc.cnr.it/lemonEty#isEtyLinkOf">
        <rdfs:domain rdf:resource="http://lari-datasets.ilc.cnr.it/lemonEty#EtyLink"/>
        <rdfs:range rdf:resource="http://lari-datasets.ilc.cnr.it/lemonEty#Etymology"/>
        <rdfs:comment xml:lang="en">&apos;is etymological link of&apos; is an object property that relates an Etymology with an Etymological Link.</rdfs:comment>
        <rdfs:label xml:lang="en">is etymological link of</rdfs:label>
    </owl:ObjectProperty>
    


    <!-- http://lari-datasets.ilc.cnr.it/lemonEty#isEtymologyOf -->

    <owl:ObjectProperty rdf:about="http://lari-datasets.ilc.cnr.it/lemonEty#isEtymologyOf">
        <rdfs:domain rdf:resource="http://lari-datasets.ilc.cnr.it/lemonEty#Etymology"/>
        <rdfs:comment xml:lang="en">&apos;is etymology of&apos; is an object property linking an Etymology with a linguistic entity.</rdfs:comment>
        <rdfs:label xml:lang="en">is etymology of</rdfs:label>
    </owl:ObjectProperty>
    


    <!-- http://lari-datasets.ilc.cnr.it/lemonEty#isEtymonOf -->

    <owl:ObjectProperty rdf:about="http://lari-datasets.ilc.cnr.it/lemonEty#isEtymonOf">
        <rdfs:domain rdf:resource="http://lari-datasets.ilc.cnr.it/lemonEty#Etymon"/>
        <rdfs:range rdf:resource="http://lari-datasets.ilc.cnr.it/lemonEty#Etymology"/>
        <rdfs:comment xml:lang="en">&apos;is etymon of&apos; is an object property that relates an Etymon with the etymologies it is a part of.</rdfs:comment>
        <rdfs:label xml:lang="en">is etymon of</rdfs:label>
    </owl:ObjectProperty>
    


    <!-- http://lari-datasets.ilc.cnr.it/lemonEty#startingLink -->

    <owl:ObjectProperty rdf:about="http://lari-datasets.ilc.cnr.it/lemonEty#startingLink">
        <rdfs:subPropertyOf rdf:resource="http://lari-datasets.ilc.cnr.it/lemonEty#hasEtyLink"/>
        <rdfs:domain rdf:resource="http://lari-datasets.ilc.cnr.it/lemonEty#Etymology"/>
        <rdfs:range rdf:resource="http://lari-datasets.ilc.cnr.it/lemonEty#EtyLink"/>
        <rdfs:comment xml:lang="en">&apos;starting link&apos; is  an object property that relates an Etymology with its first Etymological Link.</rdfs:comment>
        <rdfs:label xml:lang="en">starting link</rdfs:label>
    </owl:ObjectProperty>
    


    <!-- 
    ///////////////////////////////////////////////////////////////////////////////////////
    //
    // Data properties
    //
    ///////////////////////////////////////////////////////////////////////////////////////
     -->

    


    <!-- http://lari-datasets.ilc.cnr.it/lemonEty#etyLinkType -->

    <owl:DatatypeProperty rdf:about="http://lari-datasets.ilc.cnr.it/lemonEty#etyLinkType"/>
    


    <!-- 
    ///////////////////////////////////////////////////////////////////////////////////////
    //
    // Classes
    //
    ///////////////////////////////////////////////////////////////////////////////////////
     -->

    


    <!-- http://lari-datasets.ilc.cnr.it/lemonEty#Cognate -->

    <owl:Class rdf:about="http://lari-datasets.ilc.cnr.it/lemonEty#Cognate">
        <rdfs:subClassOf rdf:resource="http://www.w3.org/ns/lemon/ontolex#LexicalEntry"/>
        <rdfs:comment xml:lang="en">&apos;Cognate&apos; is a subclass of Lexical Entry that consists of lexemes which are cognates of another Lexical Entry.</rdfs:comment>
        <rdfs:label xml:lang="en">cognate</rdfs:label>
    </owl:Class>
    


    <!-- http://lari-datasets.ilc.cnr.it/lemonEty#EtyLink -->

    <owl:Class rdf:about="http://lari-datasets.ilc.cnr.it/lemonEty#EtyLink">
        <rdfs:comment xml:lang="en">&apos;Etymological Link&apos; is a class that consists of individuals that represent the etymological relationship between two linguistic entities.</rdfs:comment>
        <rdfs:label xml:lang="en">Etymological Link</rdfs:label>
    </owl:Class>
    


    <!-- http://lari-datasets.ilc.cnr.it/lemonEty#Etymology -->

    <owl:Class rdf:about="http://lari-datasets.ilc.cnr.it/lemonEty#Etymology">
        <rdfs:comment xml:lang="en">&apos;Etymology&apos; is a class that consists of individuals that describe the history of a Lexical Entry.</rdfs:comment>
        <rdfs:label xml:lang="en">Etymology</rdfs:label>
    </owl:Class>
    


    <!-- http://lari-datasets.ilc.cnr.it/lemonEty#Etymon -->

    <owl:Class rdf:about="http://lari-datasets.ilc.cnr.it/lemonEty#Etymon">
        <rdfs:subClassOf rdf:resource="http://www.w3.org/ns/lemon/ontolex#LexicalEntry"/>
        <rdfs:comment xml:lang="en">&apos;Etymon&apos; is a subclass of Lexical Entry that consists of invidividuals whose role is to describe the origin and history of another Lexical Entry.</rdfs:comment>
        <rdfs:label xml:lang="en">etymon</rdfs:label>
    </owl:Class>
    


    <!-- 
    ///////////////////////////////////////////////////////////////////////////////////////
    //
    // Annotations
    //
    ///////////////////////////////////////////////////////////////////////////////////////
     -->

    <rdf:Description rdf:about="http://lari-datasets.ilc.cnr.it/lemonEty#etyLinkType">
        <rdfs:comment xml:lang="en">&apos;etymological link type&apos; specifies the type of a Etymological Link.</rdfs:comment>
        <rdfs:label xml:lang="en">etymological link type</rdfs:label>
    </rdf:Description>
</rdf:RDF>



<!-- Generated by the OWL API (version 4.5.9.2019-02-01T07:24:44Z) https://github.com/owlcs/owlapi -->


